code/mpfr/MPFR.Add.Spec.fst
@@ -1,0 +1,104 @@
+module MPFR.Add.Spec
+
+open FStar.Mul
+open MPFR.Lib.Spec
+
+(* Proprieties for addition *)
+val add: a:mpfr_structP{valid_mpfr_struct a} ->
+         b:mpfr_structP{valid_mpfr_struct b /\ a.sign = b.sign} ->
+    Tot (r:mpfr_structP{r.sign = a.sign /\ r.exp >= mpfr_EMIN_spec /\ mpfr_mp_cond r /\
+          ((a.mant * pow2 (a.exp - mpfr_EMIN_spec)) +
+	   (b.mant * pow2 (b.exp - mpfr_EMIN_spec)) =
+	   (r.mant * pow2 (r.exp - mpfr_EMIN_spec)))})
+
+(* Implementation for addition *)
+private let min (a:int) (b:int) = if a >= b then b else a
+private let max (a:int) (b:int) = if a >= b then a else b
+
+val add_mant: a:mpfr_structP{valid_mpfr_struct a} ->
+              b:mpfr_structP{valid_mpfr_struct b /\ a.sign = b.sign} ->
+	  Tot nat
+let add_mant a b =
+    if a.exp >= b.exp then a.mant * pow2 (a.exp - b.exp) + b.mant
+                     else b.mant * pow2 (b.exp - a.exp) + a.mant
+    
+val add_exp : a:mpfr_structP{valid_mpfr_struct a} ->
+              b:mpfr_structP{valid_mpfr_struct b /\ a.sign = b.sign} ->
+	 Tot (r:int{r >= mpfr_EMIN_spec})
+let add_exp a b = min a.exp b.exp
+
+val add_prec: a:mpfr_structP{valid_mpfr_struct a} ->
+              b:mpfr_structP{valid_mpfr_struct b /\ a.sign = b.sign} ->
+	  Tot nat
+let add_prec a b =
+    let p0 = if a.exp >= b.exp then max (a.prec + a.exp - b.exp) b.prec 
+                              else max (b.prec + b.exp - a.exp) a.prec in
+    if add_mant a b < pow2 p0 then p0 else p0 + 1
+
+open FStar.Math.Lemmas
+
+val lemma_mult_lt_right: a:pos -> b:nat -> c:nat -> Lemma 
+    (requires b < c)
+    (ensures  b * a < c * a)
+let lemma_mult_lt_right a b c = ()
+
+(* Useful lemmas *)
+val add_mp_cond_lemma: a:mpfr_structP{valid_mpfr_struct a} ->
+                       b:mpfr_structP{valid_mpfr_struct b /\ a.sign = b.sign} ->
+    Lemma (let sp = add_prec a b in
+           let sm = add_mant a b in
+	   pow2 (sp - 1) <= sm /\ sm < pow2 sp)
+let add_mp_cond_lemma a b =
+    let sp = add_prec a b in
+    let sm = add_mant a b in
+    let p0 = if a.exp >= b.exp then max (a.prec + a.exp - b.exp) b.prec 
+                              else max (b.prec + b.exp - a.exp) a.prec in
+    if sm < pow2 p0 then begin
+	if a.exp >= b.exp then begin
+	    lemma_mult_le_right (pow2 (a.exp - b.exp)) (pow2 (a.prec - 1)) a.mant;
+	    pow2_plus (a.prec - 1) (a.exp - b.exp)
+	end else begin
+	    lemma_mult_le_right (pow2 (b.exp - a.exp)) (pow2 (b.prec - 1)) b.mant;
+	    pow2_plus (b.prec - 1) (b.exp - a.exp)
+	end
+    end else begin
+        assert(sm >= pow2 (sp - 1));
+	if a.exp >= b.exp then begin
+	    lemma_mult_lt_right (pow2 (a.exp - b.exp)) a.mant (pow2 a.prec);
+	    pow2_plus a.prec (a.exp - b.exp);
+	    pow2_le_compat (max (a.prec + a.exp - b.exp) b.prec) (a.prec + a.exp - b.exp);
+	    pow2_le_compat (max (a.prec + a.exp - b.exp) b.prec) b.prec;
+	    pow2_double_sum (max (a.prec + a.exp - b.exp) b.prec)
+	end else begin
+	    lemma_mult_lt_right (pow2 (b.exp - a.exp)) b.mant (pow2 b.prec);
+	    pow2_plus b.prec (b.exp - a.exp);
+	    pow2_le_compat (max (b.prec + b.exp - a.exp) a.prec) (b.prec + b.exp - a.exp);
+	    pow2_le_compat (max (b.prec + b.exp - a.exp) a.prec) a.prec;
+	    pow2_double_sum (max (b.prec + b.exp - a.exp) a.prec)
+	end
+    end
+
+val add_value_lemma: a:mpfr_structP{valid_mpfr_struct a} ->
+                     b:mpfr_structP{valid_mpfr_struct b /\ a.sign = b.sign} ->
+    Lemma (add_exp a b >= mpfr_EMIN_spec /\
+           (a.mant * pow2 (a.exp - mpfr_EMIN_spec)) +
+	   (b.mant * pow2 (b.exp - mpfr_EMIN_spec)) =
+	   (add_mant a b * pow2 (add_exp a b - mpfr_EMIN_spec)))
+let add_value_lemma a b = 
+    let sx = add_exp a b in
+    let sm = add_mant a b in
+    if a.exp >= b.exp then begin
+        distributivity_add_left (a.mant * pow2 (a.exp - b.exp)) b.mant (pow2 (sx - mpfr_EMIN_spec));
+	paren_mul_right a.mant (pow2 (a.exp - b.exp)) (pow2 (sx - mpfr_EMIN_spec));
+	pow2_plus (a.exp - b.exp) (sx - mpfr_EMIN_spec)
+    end else begin
+        distributivity_add_left (b.mant * pow2 (b.exp - a.exp)) a.mant (pow2 (sx - mpfr_EMIN_spec));
+	paren_mul_right b.mant (pow2 (b.exp - a.exp)) (pow2 (sx - mpfr_EMIN_spec));
+	pow2_plus (b.exp - a.exp) (sx - mpfr_EMIN_spec)
+    end
+
+let add a b = 
+    add_mp_cond_lemma a b;
+    add_value_lemma a b;
+    {sign = a.sign; prec = add_prec a b; mant = add_mant a b; exp = add_exp a b}
+
