code/mpfr/MPFR.Lib.Spec.fst
@@ -1,0 +1,29 @@
+module MPFR.Lib.Spec
+
+
+let gmp_NUMB_BITS_spec = 64
+let mpfr_PREC_MIN_spec = 1
+let mpfr_PREC_MAX_spec = gmp_NUMB_BITS_spec - 1
+let mpfr_EXP_INVALID_spec = pow2 30
+let mpfr_EMIN_spec = 1 - mpfr_EXP_INVALID_spec
+let mpfr_EMAX_spec = mpfr_EXP_INVALID_spec - 1
+let mpfr_SIGN_POS  = 1
+let mpfr_SIGN_NEG  = -1
+
+let mpfr_prec_cond (p:pos) = mpfr_PREC_MIN_spec <= p /\ p <= mpfr_PREC_MAX_spec
+let mpfr_exp_cond  (x:int) = mpfr_EMIN_spec <= x /\ x <= mpfr_EMAX_spec
+let mpfr_sign_cond (s:int) = s = mpfr_SIGN_POS \/ s = mpfr_SIGN_NEG
+
+type mpfr_structP = {
+    sign: int;
+    prec: pos;
+    mant: nat;
+    exp : int
+}
+
+let mpfr_mp_cond (s:mpfr_structP) = pow2 (s.prec - 1) <= s.mant /\ s.mant < pow2 s.prec
+
+let valid_mpfr_struct (s:mpfr_structP) =
+    mpfr_prec_cond s.prec /\ mpfr_exp_cond s.exp /\ mpfr_sign_cond s.sign /\
+    mpfr_mp_cond s
+
