code/mpfr/MPFR.Rounding.Spec.fst
@@ -1,0 +1,86 @@
+module MPFR.Rounding.Spec
+
+open FStar.UInt
+open MPFR.Lib.Spec
+
+(* Definitions of rounding bit and sticky bit *)
+let nth_bit  (#m:pos) (a:uint_t m) (n:nat) = if n < m then nth a n else false
+
+val rb_spec: a:mpfr_structP{valid_mpfr_struct a} -> p:pos{mpfr_prec_cond p} ->
+    Tot (rb:bool{rb <==> nth_bit #a.prec a.mant p})
+    
+let nth_from (#m:pos) (a:uint_t m) (n:nat) = exists (i:nat{n <= i /\ i < m}). nth a i
+
+val sb_spec: a:mpfr_structP{valid_mpfr_struct a} -> p:pos{mpfr_prec_cond p} -> 
+    Tot (sb:bool{sb <==> nth_from #a.prec a.mant (p + 1)})
+
+
+(* Useful lemmas for proving rounding/sticky bit proprieties *)		 
+let rb_spec a p =
+    if a.prec <= p then false
+    else nth #a.prec a.mant p
+    
+val bitor_from: #n:pos -> a:uint_t n -> s:nat{s < n} ->
+    Tot (b:bool{b <==> nth_from #n a s}) (decreases (n - s))
+let rec bitor_from #n a s =
+    if s + 1 = n then nth a s
+                 else nth a s || bitor_from #n a (s + 1)
+
+let sb_spec a p = 
+    if a.prec <= p + 1 then false
+    else bitor_from #a.prec a.mant (p + 1)
+
+val nth_from_plusone_lemma: #m:pos -> a:uint_t m -> n:nat{n < m} ->
+    Lemma (nth_from a n <==> (nth a n \/ nth_from a (n + 1)))
+let nth_from_plusone_lemma #m a n = ()
+
+val pow2m1_nth_lemma: #n:pos -> p:nat{p < n} -> i:nat{i < n} ->
+    Lemma (ensures (i > n - p - 1 ==> nth #n (pow2_n #n p - 1) i = true) /\
+	           (i <= n - p - 1 ==> nth #n (pow2_n #n p - 1) i = false))
+          [SMTPat (nth #n (pow2_n #n p - 1) i)]
+let pow2m1_nth_lemma #n p i = ()
+
+val logor_pow2_pow2m1_nth_lemma: #n:pos -> p:nat{p + 1 < n} -> i:nat{i < n} ->
+    Lemma (ensures (nth #n (logor (pow2_n #n p) (pow2_n #n p - 1)) i =
+                    nth #n (pow2_n #n (p + 1) - 1) i))
+          [SMTPat (nth #n (logor (pow2_n #n p) (pow2_n #n p - 1)) i)]
+let logor_pow2_pow2m1_nth_lemma #n p i = ()
+
+val logand_logor_distr: #n:pos -> a:uint_t n -> b:uint_t n -> c:uint_t n ->
+    Lemma (logand a (logor b c) = logor (logand a b) (logand a c))
+let logand_logor_distr #n a b c =
+    nth_lemma (logand a (logor b c)) (logor (logand a b) (logand a c))
+
+val logor_not_zero: #n:pos -> a:uint_t n -> b:uint_t n ->
+    Lemma (logor a b <> 0 <==> (a <> 0 \/ b <> 0))
+let logor_not_zero #n a b = if b = 0 then logor_lemma_1 a else logor_ge a b
+
+val rb_mask_lemma: #n:pos -> a:uint_t n -> s:nat{s < n} ->
+    Lemma (nth a s <==> logand a (pow2_n #n (n - s - 1)) <> 0)
+let rb_mask_lemma #n a s =
+    if nth a s then nth_lemma (logand a (pow2_n #n (n - s - 1))) (pow2_n #n (n - s - 1))
+    else nth_lemma (logand a (pow2_n #n (n - s - 1))) (zero n)
+
+val sb_mask_lemma: #n:pos -> a:uint_t n -> s:pos{s < n} ->
+    Lemma (ensures (nth_from a s <==> logand a (pow2_n #n (n - s) - 1) <> 0))
+          (decreases (n - s))
+let rec sb_mask_lemma #n a s =
+    if s + 1 = n then rb_mask_lemma a s
+    else begin
+      rb_mask_lemma #n a s;
+      sb_mask_lemma #n a (s + 1);
+      nth_from_plusone_lemma a s;
+      logor_not_zero (logand a (pow2_n #n (n - s - 1))) (logand a (pow2_n #n (n - s - 1) - 1));
+      nth_lemma (logor (pow2_n #n (n - s - 1)) (pow2_n #n (n - s - 1) - 1)) (pow2_n #n (n - s) - 1);
+      logand_logor_distr a (pow2_n #n (n - s - 1)) (pow2_n #n (n - s - 1) - 1)
+    end
+
+
+(* Proprieties of rounding bit and sticky bit *)
+val rb_spec_lemma: a:mpfr_structP{valid_mpfr_struct a} -> p:pos{mpfr_prec_cond p /\ p < a.prec} ->
+    Lemma (rb_spec a p = (logand a.mant (pow2_n #a.prec (a.prec - p - 1)) <> 0))
+let rb_spec_lemma a p = rb_mask_lemma #a.prec a.mant p
+
+val sb_spec_lemma: a:mpfr_structP{valid_mpfr_struct a} -> p:pos{mpfr_prec_cond p /\ p < a.prec - 1} ->
+    Lemma (sb_spec a p = (logand #a.prec a.mant (pow2_n #a.prec (a.prec - p - 1) - 1) <> 0))
+let sb_spec_lemma a p = sb_mask_lemma #a.prec a.mant (p + 1)
